txn-data-consistency/Prot_2PC_2PL.thy
@@ -1,0 +1,42 @@
+section \<open>Two Phase Commit (2PC) with Two Phase Locking (2PL)\<close>
+
+theory Prot_2PC_2PL
+  imports Key_Value_Stores
+begin
+
+subsection \<open>2PC Event system\<close>
+
+subsubsection \<open>State\<close>
+
+datatype status_rm = working | prepared | okay | notokay | committed | aborted |
+                     prep_uabort | user_aborted
+datatype status_tm = tm_init | tm_prepared | tm_committed | tm_aborted | tm_user_aborted
+
+record tm_state =
+  tm_status :: status_tm
+  tm_tid :: nat
+
+typedecl rmid
+
+record 'v rm_state =
+  rm_main_db :: "'v kv_store"
+  rm_shadow_db :: "'v kv_store"
+  rm_status :: status_rm
+  rm_tid :: nat
+
+type_synonym 'v rms_state = "rmid \<Rightarrow> 'v rm_state"
+
+record 'v global_state =
+  tm :: tm_state
+  rms :: "'v rms_state"
+
+
+subsubsection \<open>Events\<close>
+
+datatype ev2 = Prepare rmid | OK rmid | NOK rmid | PrepUAbort rmid |
+               UAbort rmid | Commit rmid | Abort rmid | Ready rmid |
+               User_Commit | User_Abort | TM_Commit | TM_Abort |
+               TM_ReadyC | TM_ReadyA | Skip
+
+
+end
